theories/RTac/IdtacK.v
@@ -1,0 +1,41 @@
+Require Import ExtLib.Data.Sum.
+Require Import ExtLib.Tactics.
+Require Import MirrorCore.RTac.CoreK.
+
+Require Import MirrorCore.Util.Forwardy.
+
+Set Implicit Arguments.
+Set Strict Implicit.
+
+Section parameterized.
+  Context {typ : Type}.
+  Context {expr : Type}.
+  Context {RType_typ : RType typ}.
+  Context {RTypeOk_typ : RTypeOk}.
+  Context {Typ0_Prop : Typ0 _ Prop}.
+  Context {Expr_expr : Expr RType_typ expr}.
+  Context {ExprUVar_expr : ExprUVar expr}.
+
+  Definition IDTACK : rtacK typ expr :=
+    fun _ _ _ _ ctx sub gl => More_ sub gl.
+
+  (** TODO: Move this **)
+  Lemma rtacK_spec_More_
+    : forall (ctx : Ctx typ expr) (s : ctx_subst ctx) g,
+      rtacK_spec s g (More_ s g).
+  Proof.
+    red. intros. split; auto. split; auto.
+    forward.
+    split.
+    - reflexivity.
+    - intros. eapply Pure_pctxD; eauto.
+  Qed.
+
+  Theorem IDTACK_sound : rtacK_sound IDTACK.
+  Proof.
+    unfold IDTACK, rtacK_sound.
+    intros; subst.
+    eapply rtacK_spec_More_.
+  Qed.
+
+End parameterized.
