theories/Views/ViewSumN.v
@@ -1,0 +1,103 @@
+Require Import ExtLib.Data.Map.FMapPositive.
+Require Import ExtLib.Data.SumN.
+Require Import ExtLib.Data.Positive.
+Require Import ExtLib.Tactics.
+Require Import MirrorCore.Views.Ptrns.
+Require Import MirrorCore.TypesI.
+Require Import MirrorCore.SymI.
+Require Import MirrorCore.syms.SymOneOf.
+Require Import MirrorCore.Views.FuncView.
+
+Section FuncViewSumN.
+  Context {A func : Type}.
+
+  Global Instance FuncViewPMap (p : positive) (m : FMapPositive.pmap Type)
+	 (pf : Some A = pmap_lookup' m p)
+  : FuncView (OneOf m) A :=
+  { f_insert := @Into m _ p (eq_sym pf)
+  ; f_view   :=
+      let view := @OutOf m _ _ (eq_sym pf) in
+      fun x =>
+        match view x with
+        | None => vNone
+        | Some x => vSome x
+        end
+  }.
+
+  Variable typ : Type.
+  Variable RType_typ : RType typ.
+
+  Require Import MirrorCore.Util.Compat.
+
+  Definition asNth'' ts p (x : OneOf ts)
+  : option match pmap_lookup' ts p with
+           | Some T => T
+           | None => Empty_set:Type
+           end :=
+    match Pos.eq_dec (index _ x) p with
+    | left pf' => Some match pf' in _ = X return match pmap_lookup' ts X with
+                                                 | Some T => T
+                                                 | None => Empty_set:Type
+                                                 end
+                       with
+                       | eq_refl => value _ x
+                       end
+    | right _ => None
+    end.
+
+  Theorem asNth'_asNth''
+  : forall ts p x,
+      @asNth' ts p (index _ x) (value _ x) = @asNth'' ts p x.
+  Proof using.
+    destruct x. unfold asNth''. simpl.
+    destruct (Pos.eq_dec index p); subst.
+    { revert value; revert ts.
+      induction p; simpl; intros; eauto. }
+    { revert value; revert ts; generalize dependent index.
+      induction p; destruct index; simpl; intros; eauto.
+      { assert (index <> p) by congruence.
+        eauto. }
+      { assert (index <> p) by congruence.
+        eauto. }
+      { congruence. } }
+  Qed.
+
+  Theorem Outof_Into : forall ts T p pf v,
+    @OutOf ts T p pf (@Into ts T p pf v) = Some v.
+  Proof using.
+  Admitted.
+
+  Theorem Into_OutOf : forall ts T p pf v e,
+      @OutOf ts T p pf e = Some v ->
+      @Into ts T p pf v = e.
+  Proof using.
+    unfold OutOf. unfold Into.
+    intros. revert H.
+    autorewrite_with_eq_rw.
+  Admitted.
+
+  Global Instance FuncViewOkPMap
+         (p : positive) (m : FMapPositive.pmap Type)
+         (syms : forall p : positive,
+             RSym match pmap_lookup' m p with
+                  | Some T => T
+                  | None => Empty_set
+                  end)
+	 (pf : Some A = pmap_lookup' m p)
+         (RSa : RSym A)
+  : FuncViewOk (FuncViewPMap p m pf) (RSymOneOf _ _) RSa.
+  Proof.
+    constructor.
+    { unfold f_view, f_insert; simpl.
+      clear. intros.
+      split.
+      { consider (OutOf A p (eq_sym pf) f); intros; try congruence.
+        inversion H0; clear H0; subst.
+        eauto using Into_OutOf. }
+      { intros.
+        subst.
+        rewrite OutOf_Into. reflexivity. } }
+    { admit. }
+  Admitted.
+
+End FuncViewSumN.
